#### 1

Givet: 

$$
R(s) = \frac{1}{s} \quad G(s)= \frac{10}{s+10}\\
C(s) = R(s)G(s)
$$


Derfor:

$$ 
C(s) = \frac{10}{s(s+10)} = \frac{1}{s} - \frac{1}{s+10}
$$
Dermed:
$$ c(t) = 1 - e^{-10t} $$

$$ \tau = \frac{1}{10}$$

```{r, echo = FALSE}
expr <- function(s) (10)/(s+10)
x_zero <- c()
y_zero <- c()
x_pole <- c(-10)
y_pole <- c(0)
pole_zero_plot(x_zero, y_zero, x_pole, y_pole, 15,expr,2)
```

#### 2

Givet: 

$$
R(s) = \frac{1}{s} \quad G(s)= \frac{20}{s+15}\\
C(s) = R(s)G(s)
$$



Derfor:

$$ 
C(s) = \frac{20}{s(s+15)} = \frac{\frac{20}{15}}{s} - \frac{\frac{20}{15}}{s+10}
$$
Dermed:
$$ c(t) = \frac{20}{15} \left(1 - e^{-15t}\right) $$

$$ \tau = \frac{1}{15}$$

```{r, echo = FALSE}
expr <- function(s) (20)/(s+15)
x_zero <- c()
y_zero <- c()
x_pole <- c(-15)
y_pole <- c(0)
pole_zero_plot(x_zero, y_zero, x_pole, y_pole, 20,expr,2)

```